Progress proof

src/MicroSail.v
@@ -1,6 +1,7 @@
 Require Export Coq.Unicode.Utf8.
 Require Import Coq.ZArith.ZArith.
 Require Import Coq.Strings.String.
+Require Import Coq.Program.Tactics.
 
 Set Implicit Arguments.
 
@@ -146,7 +147,6 @@ Module Type TermKit (typeKit : TypeKit).
 
   (* Names of expression variables. *)
   Parameter 𝑿 : Set. (* input: \MIX *)
-  Parameter 𝑿_eq_dec : forall x y : 𝑿, {x=y}+{~x=y}.
   (* Names of functions. *)
   Parameter 𝑭  : Set.
   Parameter pi : 𝑭 → FunTy.
@@ -155,8 +155,16 @@ Module Type TermKit (typeKit : TypeKit).
 
     Inductive Bit : Set := bitzero | bitone.
 
-    Inductive TaggedLit : Ty -> Set :=
-    | taglit_union (T : 𝑻) (K : 𝑲 T) : TaggedLit (𝑲_Ty K) -> TaggedLit (ty_union T)
+    Inductive TaggedLit : Ty → Set :=
+    | taglit_int           : Z → TaggedLit (ty_int)
+    | taglit_bool          : bool → TaggedLit (ty_bool)
+    | taglit_bit           : Bit → TaggedLit (ty_bit)
+    | taglit_string        : string → TaggedLit (ty_string)
+    | taglit_list   σ'     : list (TaggedLit σ') → TaggedLit (ty_list σ')
+    | taglit_prod   σ₁ σ₂  : TaggedLit σ₁ * TaggedLit σ₂ → TaggedLit (ty_prod σ₁ σ₂)
+    | taglit_sum    σ₁ σ₂  : TaggedLit σ₁ + TaggedLit σ₂ → TaggedLit (ty_sum σ₁ σ₂)
+    | taglit_unit          : TaggedLit (ty_unit)
+    | taglit_union (T : 𝑻) (K : 𝑲 T) : TaggedLit (𝑲_Ty K) → TaggedLit (ty_union T)
     | taglit_record (R : 𝑹) : Env TaggedLit (𝑹𝑭_Ty R) -> TaggedLit (ty_record R).
 
     Fixpoint Lit (σ : Ty) : Set :=
@@ -175,15 +183,140 @@ Module Type TermKit (typeKit : TypeKit).
 
     Fixpoint untag {σ : Ty} (v : TaggedLit σ) : Lit σ :=
       match v with
-      | taglit_union v => existT _ _ v
-      | taglit_record t => t
+      | taglit_int  z       => z
+      | taglit_bool b       => b
+      | taglit_bit b        => b
+      | taglit_string s     => s
+      | taglit_list ls      => List.map untag ls
+      | taglit_prod (l , r) => (untag l , untag r)
+      | taglit_sum (inl v)  => inl (untag v)
+      | taglit_sum (inr v)  => inr (untag v)
+      | taglit_unit         => tt
+      | taglit_union l      => existT _ _ l
+      | taglit_record t     => t
       end.
 
     Definition LocalStore (Γ : Ctx (𝑿 * Ty)) : Set := Env Lit Γ.
 
   End Literals.
 
+  Section Expressions.
+
+    Inductive Exp (Γ : Ctx (𝑿 * Ty)) : Ty -> Set :=
+    | exp_var     (x : 𝑿) (σ : Ty) {xInΓ : InCtx (x , σ) Γ} : Exp Γ σ
+    | exp_lit     (σ : Ty) : Lit σ → Exp Γ σ
+    | exp_plus    (e₁ e₂ : Exp Γ ty_int) : Exp Γ ty_int
+    | exp_times   (e₁ e₂ : Exp Γ ty_int) : Exp Γ ty_int
+    | exp_minus   (e₁ e₂ : Exp Γ ty_int) : Exp Γ ty_int
+    | exp_neg     (e : Exp Γ ty_int) : Exp Γ ty_int
+    | exp_eq      (e₁ e₂ : Exp Γ ty_int) : Exp Γ ty_bool
+    | exp_le      (e₁ e₂ : Exp Γ ty_int) : Exp Γ ty_bool
+    | exp_lt      (e₁ e₂ : Exp Γ ty_int) : Exp Γ ty_bool
+    | exp_and     (e₁ e₂ : Exp Γ ty_bool) : Exp Γ ty_bool
+    | exp_not     (e : Exp Γ ty_bool) : Exp Γ ty_bool
+    | exp_pair    {σ₁ σ₂ : Ty} (e₁ : Exp Γ σ₁) (e₂ : Exp Γ σ₂) : Exp Γ (ty_prod σ₁ σ₂)
+    | exp_inl     {σ₁ σ₂ : Ty} : Exp Γ σ₁ → Exp Γ (ty_sum σ₁ σ₂)
+    | exp_inr     {σ₁ σ₂ : Ty} : Exp Γ σ₂ → Exp Γ (ty_sum σ₁ σ₂)
+    | exp_list    {σ : Ty} (es : list (Exp Γ σ)) : Exp Γ (ty_list σ)
+    | exp_cons    {σ : Ty} (h : Exp Γ σ) (t : Exp Γ (ty_list σ)) : Exp Γ (ty_list σ)
+    | exp_nil     {σ : Ty} : Exp Γ (ty_list σ)
+    | exp_union   {T : 𝑻} (K : 𝑲 T) (e : Exp Γ (𝑲_Ty K)) : Exp Γ (ty_union T)
+    | exp_record  (R : 𝑹) (es : Env (Exp Γ) (𝑹𝑭_Ty R)) : Exp Γ (ty_record R)
+    | exp_builtin {σ τ : Ty} (f : Lit σ → Lit τ) (e : Exp Γ σ) : Exp Γ τ.
+
+    Global Arguments exp_union {_ _} _ _.
+    Global Arguments exp_record {_} _ _.
+
+    Fixpoint evalTagged {Γ : Ctx (𝑿 * Ty)} {σ : Ty} (e : Exp Γ σ) (δ : LocalStore Γ) {struct e} : TaggedLit σ.
+    Admitted.
+
+    Fixpoint eval {Γ : Ctx (𝑿 * Ty)} {σ : Ty} (e : Exp Γ σ) (δ : LocalStore Γ) {struct e} : Lit σ :=
+      match e in (Exp _ t) return (Lit t) with
+      | @exp_var _ x _ xInΓ => env_lookup δ xInΓ
+      | exp_lit _ _ l       => l
+      | exp_plus e₁ e2      => Z.add (eval e₁ δ) (eval e2 δ)
+      | exp_times e₁ e2     => Z.mul (eval e₁ δ) (eval e2 δ)
+      | exp_minus e₁ e2     => Z.sub (eval e₁ δ) (eval e2 δ)
+      | exp_neg e           => Z.opp (eval e δ)
+      | exp_eq e₁ e2        => Zeq_bool (eval e₁ δ) (eval e2 δ)
+      | exp_le e₁ e2        => Z.leb (eval e₁ δ) (eval e2 δ)
+      | exp_lt e₁ e2        => Z.ltb (eval e₁ δ) (eval e2 δ)
+      | exp_and e₁ e2       => andb (eval e₁ δ) (eval e2 δ)
+      | exp_not e           => negb (eval e δ)
+      | exp_pair e₁ e2      => pair (eval e₁ δ) (eval e2 δ)
+      | exp_inl e           => inl (eval e δ)
+      | exp_inr e           => inr (eval e δ)
+      | exp_list es         => List.map (fun e => eval e δ) es
+      | exp_cons e₁ e2      => cons (eval e₁ δ) (eval e2 δ)
+      | exp_nil _           => nil
+      | exp_union K e       => existT _ K (evalTagged e δ)
+      | exp_record R es     => fun rf τ rfIn => evalTagged (es rf τ rfIn) δ
+      | exp_builtin f e     => f (eval e δ)
+      end.
+
+  End Expressions.
+
+  Section Statements.
+
+    Inductive RecordPat : Ctx (𝑹𝑭 * Ty) -> Ctx (𝑿 * Ty) -> Set :=
+    | pat_nil  : RecordPat ctx_nil ctx_nil
+    | pat_cons
+        {rfs : Ctx (𝑹𝑭 * Ty)} {Δ : Ctx (𝑿 * Ty)}
+        (pat : RecordPat rfs Δ) (rf : 𝑹𝑭) {τ : Ty} (x : 𝑿) :
+        RecordPat (ctx_snoc rfs (rf , τ)) (ctx_snoc Δ (x , τ)).
+
+    Inductive Stm (Γ : Ctx (𝑿 * Ty)) : Ty → Set :=
+    | stm_lit        {τ : Ty} (l : Lit τ) : Stm Γ τ
+    | stm_exp        {τ : Ty} (e : Exp Γ τ) : Stm Γ τ
+    | stm_let        (x : 𝑿) (τ : Ty) (s : Stm Γ τ) {σ : Ty} (k : Stm (ctx_snoc Γ (x , τ)) σ) : Stm Γ σ
+    | stm_let'       (Δ : Ctx (𝑿 * Ty)) (δ : LocalStore Δ) {σ : Ty} (k : Stm (ctx_cat Γ Δ) σ) : Stm Γ σ
+    | stm_assign     (x : 𝑿) (τ : Ty) {xInΓ : InCtx (x , τ) Γ} (e : Exp Γ τ) : Stm Γ τ
+    | stm_app        (f : 𝑭) (e : Exp Γ (fun_dom (pi f))) : Stm Γ (fun_cod (pi f))
+    | stm_app'       (x : 𝑿) (σ τ : Ty) (v : Lit σ) (s : Stm (ctx_snoc ctx_nil (x , σ)) τ) : Stm Γ τ
+    | stm_if         {τ : Ty} (e : Exp Γ ty_bool) (s₁ s₂ : Stm Γ τ) : Stm Γ τ
+    | stm_seq        {τ : Ty} (e : Stm Γ τ) {σ : Ty} (k : Stm Γ σ) : Stm Γ σ
+    | stm_assert     (e₁ : Exp Γ ty_bool) (e₂ : Exp Γ ty_string) : Stm Γ ty_bool
+    (* | stm_while      (w : 𝑾 Γ) (e : Exp Γ ty_bool) {σ : Ty} (s : Stm Γ σ) → Stm Γ ty_unit *)
+    | stm_exit       (τ : Ty) (s : Lit ty_string) : Stm Γ τ
+    | stm_match_list {σ τ : Ty} (e : Exp Γ (ty_list σ)) (alt_nil : Stm Γ τ)
+      (xh xt : 𝑿) (alt_cons : Stm (ctx_snoc (ctx_snoc Γ (xh , σ)) (xt , ty_list σ)) τ) : Stm Γ τ
+    | stm_match_sum  {σinl σinr τ : Ty} (e : Exp Γ (ty_sum σinl σinr))
+      (xinl : 𝑿) (alt_inl : Stm (ctx_snoc Γ (xinl , σinl)) τ)
+      (xinr : 𝑿) (alt_inr : Stm (ctx_snoc Γ (xinr , σinr)) τ) : Stm Γ τ
+    | stm_match_pair {σ₁ σ₂ τ : Ty} (e : Exp Γ (ty_prod σ₁ σ₂))
+      (xl xr : 𝑿) (rhs : Stm (ctx_snoc (ctx_snoc Γ (xl , σ₁)) (xr , σ₂)) τ) : Stm Γ τ
+    | stm_match_union {T : 𝑻} (e : Exp Γ (ty_union T)) {τ : Ty}
+      (alts : forall (K : 𝑲 T), { x : 𝑿 & Stm (ctx_snoc Γ (x , 𝑲_Ty K)) τ}) : Stm Γ τ
+    | stm_match_record {R : 𝑹} {Δ : Ctx (𝑿 * Ty)} (e : Exp Γ (ty_record R))
+      (p : RecordPat (𝑹𝑭_Ty R) Δ) {τ : Ty} (rhs : Stm (ctx_cat Γ Δ) τ) : Stm Γ τ.
+
+    Global Arguments stm_lit {_} _ _.
+    Global Arguments stm_exp {_ _} _.
+    Global Arguments stm_let {_} _ _ _ {_} _.
+    Global Arguments stm_let' {_ _} _ {_} _.
+    Global Arguments stm_assign {_} _ {_ _} _.
+    Global Arguments stm_app {_} _ _.
+    Global Arguments stm_app' {_} _ _ _ _ _.
+    Global Arguments stm_if {_ _} _ _ _.
+    Global Arguments stm_seq {_ _} _ {_} _.
+    Global Arguments stm_assert {_} _ _.
+    Global Arguments stm_exit {_} _ _.
+    Global Arguments stm_match_list {_ _ _} _ _ _ _ _.
+    Global Arguments stm_match_sum {_ _ _ _} _ _ _ _ _.
+    Global Arguments stm_match_pair {_ _ _ _} _ _ _ _.
+    Global Arguments stm_match_union {_ _} _ {_} _.
+    Global Arguments stm_match_record {_} _ {_} _ _ {_} _.
+
+  End Statements.
+
+  Record FunDef (fty : FunTy) : Set :=
+    { fun_arg  : 𝑿;
+      fun_body : Stm (ctx_snoc ctx_nil (fun_arg , fun_dom fty)) (fun_cod fty)
+    }.
+
   Module NameResolution.
+
+    Parameter 𝑿_eq_dec : forall x y : 𝑿, {x=y}+{~x=y}.
 
     Fixpoint ctx_resolve {D : Set} (Γ : Ctx (𝑿 * D)) (x : 𝑿) {struct Γ} : option D :=
       match Γ with
@@ -216,130 +349,14 @@ Module Type TermKit (typeKit : TypeKit).
         end
       end.
 
-  End NameResolution.
-
-  Section Expressions.
-
-    Inductive Exp (Γ : Ctx (𝑿 * Ty)) : Ty -> Set :=
-    | exp_var    (x : 𝑿) (σ : Ty) {xInΓ : InCtx (x , σ) Γ} : Exp Γ σ
-    | exp_lit    (σ : Ty) : Lit σ → Exp Γ σ
-    | exp_plus   (e₁ e₂ : Exp Γ ty_int) : Exp Γ ty_int
-    | exp_times  (e₁ e₂ : Exp Γ ty_int) : Exp Γ ty_int
-    | exp_minus  (e₁ e₂ : Exp Γ ty_int) : Exp Γ ty_int
-    | exp_neg    (e : Exp Γ ty_int) : Exp Γ ty_int
-    | exp_eq     (e₁ e₂ : Exp Γ ty_int) : Exp Γ ty_bool
-    | exp_le     (e₁ e₂ : Exp Γ ty_int) : Exp Γ ty_bool
-    | exp_lt     (e₁ e₂ : Exp Γ ty_int) : Exp Γ ty_bool
-    | exp_and    (e₁ e₂ : Exp Γ ty_bool) : Exp Γ ty_bool
-    | exp_not    (e : Exp Γ ty_bool) : Exp Γ ty_bool
-    | exp_pair   {σ₁ σ₂ : Ty} (e₁ : Exp Γ σ₁) (e₂ : Exp Γ σ₂) : Exp Γ (ty_prod σ₁ σ₂)
-    | exp_inl    {σ₁ σ₂ : Ty} : Exp Γ σ₁ → Exp Γ (ty_sum σ₁ σ₂)
-    | exp_inr    {σ₁ σ₂ : Ty} : Exp Γ σ₂ → Exp Γ (ty_sum σ₁ σ₂)
-    | exp_list   {σ : Ty} (es : list (Exp Γ σ)) : Exp Γ (ty_list σ)
-    | exp_cons   {σ : Ty} (h : Exp Γ σ) (t : Exp Γ (ty_list σ)) : Exp Γ (ty_list σ)
-    | exp_nil    {σ : Ty} : Exp Γ (ty_list σ)
-    | exp_union  {T : 𝑻} (K : 𝑲 T) (e : Exp Γ (𝑲_Ty K)) : Exp Γ (ty_union T)
-    | exp_record (R : 𝑹) (es : Env (Exp Γ) (𝑹𝑭_Ty R)) : Exp Γ (ty_record R).
-
-    Global Arguments exp_union {_ _} _ _.
-    Global Arguments exp_record {_} _ _.
-
-    Import NameResolution.
-
     Definition exp_smart_var {Γ : Ctx (𝑿 * Ty)} (x : 𝑿) {p : IsSome (ctx_resolve Γ x)} :
       Exp Γ (fromSome (ctx_resolve Γ x) p) := @exp_var Γ x (fromSome _ p) (mk_inctx Γ x p).
-
-    Fixpoint evalTagged {Γ : Ctx (𝑿 * Ty)} {σ : Ty} (e : Exp Γ σ) (δ : LocalStore Γ) {struct e} : TaggedLit σ.
-    Admitted.
-
-    Fixpoint eval {Γ : Ctx (𝑿 * Ty)} {σ : Ty} (e : Exp Γ σ) (δ : LocalStore Γ) {struct e} : Lit σ :=
-      match e in (Exp _ t) return (Lit t) with
-      | @exp_var _ x _ xInΓ => env_lookup δ xInΓ
-      | exp_lit _ _ l       => l
-      | exp_plus e₁ e2      => Z.add (eval e₁ δ) (eval e2 δ)
-      | exp_times e₁ e2     => Z.mul (eval e₁ δ) (eval e2 δ)
-      | exp_minus e₁ e2     => Z.sub (eval e₁ δ) (eval e2 δ)
-      | exp_neg e           => Z.opp (eval e δ)
-      | exp_eq e₁ e2        => Zeq_bool (eval e₁ δ) (eval e2 δ)
-      | exp_le e₁ e2        => Z.leb (eval e₁ δ) (eval e2 δ)
-      | exp_lt e₁ e2        => Z.ltb (eval e₁ δ) (eval e2 δ)
-      | exp_and e₁ e2       => andb (eval e₁ δ) (eval e2 δ)
-      | exp_not e           => negb (eval e δ)
-      | exp_pair e₁ e2      => pair (eval e₁ δ) (eval e2 δ)
-      | exp_inl e           => inl (eval e δ)
-      | exp_inr e           => inr (eval e δ)
-      | exp_list es         => List.map (fun e => eval e δ) es
-      | exp_cons e₁ e2      => cons (eval e₁ δ) (eval e2 δ)
-      | exp_nil _           => nil
-      | exp_union K e       => existT _ K (evalTagged e δ)
-      | exp_record R es     => fun rf τ rfIn => evalTagged (es rf τ rfIn) δ
-      end.
-
-  End Expressions.
-
-  Section Statements.
-
-    Inductive RecordPat : Ctx (𝑹𝑭 * Ty) -> Ctx (𝑿 * Ty) -> Set :=
-    | pat_nil  : RecordPat ctx_nil ctx_nil
-    | pat_cons
-        {rfs : Ctx (𝑹𝑭 * Ty)} {Δ : Ctx (𝑿 * Ty)}
-        (pat : RecordPat rfs Δ) (rf : 𝑹𝑭) {τ : Ty} (x : 𝑿) :
-        RecordPat (ctx_snoc rfs (rf , τ)) (ctx_snoc Δ (x , τ)).
-
-    Inductive Stm (Γ : Ctx (𝑿 * Ty)) : Ty → Set :=
-    | stm_lit        {τ : Ty} (l : Lit τ) : Stm Γ τ
-    | stm_exp        {τ : Ty} (e : Exp Γ τ) : Stm Γ τ
-    | stm_let        (x : 𝑿) (τ : Ty) (s : Stm Γ τ) {σ : Ty} (k : Stm (ctx_snoc Γ (x , τ)) σ) : Stm Γ σ
-    | stm_let'       (Δ : Ctx (𝑿 * Ty)) (δ : Env Lit Δ) {σ : Ty} (k : Stm (ctx_cat Γ Δ) σ) : Stm Γ σ
-    | stm_assign     (x : 𝑿) (τ : Ty) {xInΓ : InCtx (x , τ) Γ} (e : Exp Γ τ) : Stm Γ τ
-    | stm_app        (f : 𝑭) (e : Exp Γ (fun_dom (pi f))) : Stm Γ (fun_cod (pi f))
-    | stm_app'       (x : 𝑿) (σ τ : Ty) (v : Lit σ) (s : Stm (ctx_snoc ctx_nil (x , σ)) τ) : Stm Γ τ
-    | stm_if         {τ : Ty} (e : Exp Γ ty_bool) (s₁ s₂ : Stm Γ τ) : Stm Γ τ
-    | stm_seq        {τ : Ty} (e : Stm Γ τ) {σ : Ty} (k : Stm Γ σ) : Stm Γ σ
-    | stm_assert     (e₁ : Exp Γ ty_bool) (e₂ : Exp Γ ty_string) : Stm Γ ty_bool
-    (* | stm_while      (w : 𝑾 Γ) (e : Exp Γ ty_bool) {σ : Ty} (s : Stm Γ σ) → Stm Γ ty_unit *)
-    | stm_exit       {τ : Ty} (s : Lit ty_string) : Stm Γ τ
-    | stm_match_list {σ τ : Ty} (e : Exp Γ (ty_list σ)) (alt_nil : Stm Γ τ)
-      (xh xt : 𝑿) (alt_cons : Stm (ctx_snoc (ctx_snoc Γ (xh , σ)) (xt , ty_list σ)) τ) : Stm Γ τ
-    | stm_match_sum  {σinl σinr τ : Ty} (e : Exp Γ (ty_sum σinl σinr))
-      (xinl : 𝑿) (alt_inl : Stm (ctx_snoc Γ (xinl , σinl)) τ)
-      (xinr : 𝑿) (alt_inr : Stm (ctx_snoc Γ (xinr , σinr)) τ) : Stm Γ τ
-    | stm_match_pair {σ₁ σ₂ τ : Ty} (e : Exp Γ (ty_prod σ₁ σ₂))
-      (xl xr : 𝑿) (rhs : Stm (ctx_snoc (ctx_snoc Γ (xl , σ₁)) (xr , σ₂)) τ) : Stm Γ τ
-    | stm_match_union {T : 𝑻} (e : Exp Γ (ty_union T)) {τ : Ty}
-      (alts : forall (K : 𝑲 T), { x : 𝑿 & Stm (ctx_snoc Γ (x , 𝑲_Ty K)) τ}) : Stm Γ τ
-    | stm_match_record {R : 𝑹} {Δ : Ctx (𝑿 * Ty)} (e : Exp Γ (ty_record R))
-      (p : RecordPat (𝑹𝑭_Ty R) Δ) {τ : Ty} (rhs : Stm (ctx_cat Γ Δ) τ) : Stm Γ τ.
-
-    Global Arguments stm_lit {_} _ _.
-    Global Arguments stm_exp {_ _} _.
-    Global Arguments stm_let {_} _ _ _ {_} _.
-    Global Arguments stm_let' {_ _} _ {_} _.
-    Global Arguments stm_assign {_} _ {_ _} _.
-    Global Arguments stm_app {_} _ _.
-    Global Arguments stm_app' {_} _ _ _ _ _.
-    Global Arguments stm_if {_ _} _ _ _.
-    Global Arguments stm_seq {_ _} _ {_} _.
-    Global Arguments stm_assert {_} _ _.
-    Global Arguments stm_exit {_ _} _.
-    Global Arguments stm_match_list {_ _ _} _ _ _ _ _.
-    Global Arguments stm_match_sum {_ _ _ _} _ _ _ _ _.
-    Global Arguments stm_match_pair {_ _ _ _} _ _ _ _.
-    Global Arguments stm_match_union {_ _} _ {_} _.
-    Global Arguments stm_match_record {_} _ {_} _ _ {_} _.
-
-    Import NameResolution.
 
     Definition stm_smart_assign {Γ : Ctx (𝑿 * Ty)} (x : 𝑿) {p : IsSome (ctx_resolve Γ x)} :
       Exp Γ (fromSome (ctx_resolve Γ x) p) → Stm Γ (fromSome (ctx_resolve Γ x) p) :=
       @stm_assign Γ x (fromSome _ p) (mk_inctx Γ x p).
 
-  End Statements.
-
-  Record FunDef (fty : FunTy) : Set :=
-    { fun_arg  : 𝑿;
-      fun_body : Stm (ctx_snoc ctx_nil (fun_arg , fun_dom fty)) (fun_cod fty)
-    }.
+  End NameResolution.
 
 End TermKit.
 
@@ -361,17 +378,17 @@ Module Type ProgramKit (typeKit : TypeKit) (termKit : TermKit typeKit).
                (untag (E rf _ inctx_zero))
       end.
 
-    Record State (Γ : Ctx (𝑿 * Ty)) (σ : Ty) : Set :=
-      { state_local_store : LocalStore Γ;
-        state_statement   : Stm Γ σ
-      }.
+    (* Record State (Γ : Ctx (𝑿 * Ty)) (σ : Ty) : Set := *)
+    (*   { state_local_store : LocalStore Γ; *)
+    (*     state_statement   : Stm Γ σ *)
+    (*   }. *)
 
-    Notation "'⟨' δ ',' s '⟩'" := {| state_local_store := δ; state_statement := s |}.
-    Reserved Notation "st₁ ---> st₂" (at level 80).
+    (* Notation "'⟨' δ ',' s '⟩'" := {| state_local_store := δ; state_statement := s |}. *)
+    Reserved Notation "'⟨' δ1 ',' s1 '⟩' '--->' '⟨' δ2 ',' s2 '⟩'" (at level 80).
 
     Import NameNotation.
 
-    Inductive step {Γ : Ctx (𝑿 * Ty)} : forall {σ : Ty} (st₁ st₂ : State Γ σ), Prop :=
+    Inductive Step {Γ : Ctx (𝑿 * Ty)} : forall {σ : Ty} (δ₁ δ₂ : LocalStore Γ) (s₁ s₂ : Stm Γ σ), Prop :=
 
     | step_stm_exp
         (δ : LocalStore Γ) (σ : Ty) (e : Exp Γ σ) :
@@ -385,6 +402,9 @@ Module Type ProgramKit (typeKit : TypeKit) (termKit : TermKit typeKit).
     | step_stm_let_value
         (δ : LocalStore Γ) (x : 𝑿) (τ σ : Ty) (v : Lit τ) (k : Stm (Γ ▻ (x , τ)) σ) :
         ⟨ δ , stm_let x τ (stm_lit τ v) k ⟩ ---> ⟨ δ , stm_let' (env_nil ► x∶τ ↦ v) k ⟩
+    | step_stm_let_exit
+        (δ : LocalStore Γ) (x : 𝑿) (τ σ : Ty) (s : string) (k : Stm (Γ ▻ (x , τ)) σ) :
+        ⟨ δ , stm_let x τ (stm_exit τ s) k ⟩ ---> ⟨ δ , stm_exit σ s ⟩
     | step_stm_let'_step
         (δ δ' : LocalStore Γ) (Δ : Ctx (𝑿 * Ty)) (δΔ δΔ' : LocalStore Δ) (σ : Ty) (k k' : Stm (Γ ▻▻ Δ) σ) :
         ⟨ δ ►► δΔ , k ⟩ ---> ⟨ δ' ►► δΔ' , k' ⟩ →
@@ -392,6 +412,9 @@ Module Type ProgramKit (typeKit : TypeKit) (termKit : TermKit typeKit).
     | step_stm_let'_value
         (δ : LocalStore Γ) (Δ : Ctx (𝑿 * Ty)) (δΔ : LocalStore Δ) (σ : Ty) (v : Lit σ) :
         ⟨ δ , stm_let' δΔ (stm_lit σ v) ⟩ ---> ⟨ δ , stm_lit σ v ⟩
+    | step_stm_let'_exit
+        (δ : LocalStore Γ) (Δ : Ctx (𝑿 * Ty)) (δΔ : LocalStore Δ) (σ : Ty) (s : string) :
+        ⟨ δ , stm_let' δΔ (stm_exit σ s) ⟩ ---> ⟨ δ , stm_exit σ s ⟩
 
     | step_stm_seq_step
         (δ δ' : LocalStore Γ) (τ σ : Ty) (s s' : Stm Γ τ) (k : Stm Γ σ) :
@@ -400,6 +423,9 @@ Module Type ProgramKit (typeKit : TypeKit) (termKit : TermKit typeKit).
     | step_stm_seq_value
         (δ : LocalStore Γ) (τ σ : Ty) (v : Lit τ) (k : Stm Γ σ) :
         ⟨ δ , stm_seq (stm_lit τ v) k ⟩ ---> ⟨ δ , k ⟩
+    | step_stm_seq_exit
+        (δ : LocalStore Γ) (τ σ : Ty) (s : string) (k : Stm Γ σ) :
+        ⟨ δ , stm_seq (stm_exit τ s) k ⟩ ---> ⟨ δ , stm_exit σ s ⟩
 
     | step_stm_app
         {δ : LocalStore Γ} {f : 𝑭} (e : Exp Γ (fun_dom (pi f))) :
@@ -417,66 +443,58 @@ Module Type ProgramKit (typeKit : TypeKit) (termKit : TermKit typeKit).
     | step_stm_app'_value
       {δ : LocalStore Γ} (x : 𝑿) (σ τ : Ty) (v : Lit σ) (r : Lit τ) :
       ⟨ δ , stm_app' x σ τ v (stm_lit τ r) ⟩ ---> ⟨ δ , stm_lit τ r ⟩
+    | step_stm_app'_exit
+      {δ : LocalStore Γ} (x : 𝑿) (σ τ : Ty) (v : Lit σ) (s : string) :
+      ⟨ δ , stm_app' x σ τ v (stm_exit τ s) ⟩ ---> ⟨ δ , stm_exit τ s ⟩
 
     | step_stm_assign
         (δ : LocalStore Γ) (x : 𝑿) (σ : Ty) {xInΓ : InCtx (x , σ) Γ} (e : Exp Γ σ) :
-        ⟨ δ , stm_assign x e ⟩ ---> ⟨ δ [ x ↦ eval e δ ] , stm_lit σ (eval e δ) ⟩
+        let v := eval e δ in
+        ⟨ δ , stm_assign x e ⟩ ---> ⟨ δ [ x ↦ v ] , stm_lit σ v ⟩
     | step_stm_if
         (δ : LocalStore Γ) (e : Exp Γ ty_bool) (σ : Ty) (s₁ s₂ : Stm Γ σ) :
         ⟨ δ , stm_if e s₁ s₂ ⟩ ---> ⟨ δ , if eval e δ then s₁ else s₂ ⟩
-    | step_stm_assert_true
+    | step_stm_assert
         (δ : LocalStore Γ) (e₁ : Exp Γ ty_bool) (e₂ : Exp Γ ty_string) :
-        eval e₁ δ = true →
-        ⟨ δ , stm_assert e₁ e₂ ⟩ ---> ⟨ δ , stm_lit ty_bool true ⟩
-    | step_stm_assert_false
-        (δ : LocalStore Γ) (e₁ : Exp Γ ty_bool) (e₂ : Exp Γ ty_string) :
-        eval e₁ δ = false ->
-        ⟨ δ , stm_assert e₁ e₂ ⟩ ---> ⟨ δ , stm_exit (eval e₂ δ) ⟩
+        ⟨ δ , stm_assert e₁ e₂ ⟩ --->
+        ⟨ δ , if eval e₁ δ then stm_lit ty_bool true else stm_exit ty_bool (eval e₂ δ) ⟩
     (* | step_stm_while : *)
     (*   (δ : LocalStore Γ) (w : 𝑾 δ) (e : Exp Γ ty_bool) {σ : Ty} (s : Stm Γ σ) → *)
     (*   ⟨ δ , stm_while w e s ⟩ ---> *)
     (*   ⟨ δ , stm_if e (stm_seq s (stm_while w e s)) (stm_lit tt) ⟩ *)
-    | step_stm_match_list_nil
+    | step_stm_match_list
         (δ : LocalStore Γ) {σ τ : Ty} (e : Exp Γ (ty_list σ)) (alt_nil : Stm Γ τ)
         (xh xt : 𝑿) (alt_cons : Stm (Γ ▻ (xh , σ) ▻ (xt , ty_list σ)) τ) :
-        eval e δ = nil ->
-        ⟨ δ , stm_match_list e alt_nil xh xt alt_cons ⟩ ---> ⟨ δ , alt_nil ⟩
-    | step_stm_match_list_cons
-        (δ : LocalStore Γ) {σ τ : Ty} (e : Exp Γ (ty_list σ)) (alt_nil : Stm Γ τ)
-        (xh xt : 𝑿) (alt_cons : Stm (Γ ▻ (xh , σ) ▻ (xt , ty_list σ)) τ)
-        (vh : Lit σ) (vt : Lit (ty_list σ)) :
-        eval e δ = cons vh vt →
         ⟨ δ , stm_match_list e alt_nil xh xt alt_cons ⟩ --->
-        ⟨ δ , stm_let' (env_nil ► xh∶σ ↦ vh ► xt∶ty_list σ ↦ vt) alt_cons ⟩
-    | step_stm_match_sum_inl
+        ⟨ δ , match eval e δ with
+              | nil => alt_nil
+              | cons vh vt => stm_let' (env_nil ► xh∶σ ↦ vh ► xt∶ty_list σ ↦ vt) alt_cons
+              end
+        ⟩
+    | step_stm_match_sum
         (δ : LocalStore Γ) {σinl σinr τ : Ty} (e : Exp Γ (ty_sum σinl σinr))
         (xinl : 𝑿) (alt_inl : Stm (Γ ▻ (xinl , σinl)) τ)
-        (xinr : 𝑿) (alt_inr : Stm (Γ ▻ (xinr , σinr)) τ)
-        (v : Lit σinl) :
-        eval e δ = inl v →
+        (xinr : 𝑿) (alt_inr : Stm (Γ ▻ (xinr , σinr)) τ) :
         ⟨ δ , stm_match_sum e xinl alt_inl xinr alt_inr ⟩ --->
-        ⟨ δ , stm_let' (env_nil ► xinl∶σinl ↦ v) alt_inl ⟩
-    | step_stm_match_sum_inr
-        (δ : LocalStore Γ) {σinl σinr τ : Ty} (e : Exp Γ (ty_sum σinl σinr))
-        (xinl : 𝑿) (alt_inl : Stm (Γ ▻ (xinl , σinl)) τ)
-        (xinr : 𝑿) (alt_inr : Stm (Γ ▻ (xinr , σinr)) τ)
-        (v : Lit σinr) :
-        eval e δ = inr v →
-        ⟨ δ , stm_match_sum e xinl alt_inl xinr alt_inr ⟩ --->
-        ⟨ δ , stm_let' (env_nil ► xinr∶σinr ↦ v) alt_inr ⟩
+        ⟨ δ , match eval e δ with
+              | inl v => stm_let' (env_nil ► xinl∶σinl ↦ v) alt_inl
+              | inr v => stm_let' (env_nil ► xinr∶σinr ↦ v) alt_inr
+              end
+        ⟩
     | step_stm_match_pair
         (δ : LocalStore Γ) {σ₁ σ₂ τ : Ty} (e : Exp Γ (ty_prod σ₁ σ₂)) (xl xr : 𝑿)
-        (rhs : Stm (Γ ▻ (xl , σ₁) ▻ (xr , σ₂)) τ) (vl : Lit σ₁) (vr : Lit σ₂) :
-        eval e δ = (vl , vr) →
+        (rhs : Stm (Γ ▻ (xl , σ₁) ▻ (xr , σ₂)) τ) :
         ⟨ δ , stm_match_pair e xl xr rhs ⟩ --->
-        ⟨ δ , stm_let' (env_nil ► xl∶σ₁ ↦ vl ► xr∶σ₂ ↦ vr) rhs ⟩
+        ⟨ δ , let (vl , vr) := eval e δ in
+              stm_let' (env_nil ► xl∶σ₁ ↦ vl ► xr∶σ₂ ↦ vr) rhs
+        ⟩
     | step_stm_match_union
         (δ : LocalStore Γ) {T : 𝑻} (e : Exp Γ (ty_union T)) {τ : Ty}
-        (alts : forall (K : 𝑲 T), { x : 𝑿 & Stm (ctx_snoc Γ (x , 𝑲_Ty K)) τ})
-        (K : 𝑲 T) (v : TaggedLit (𝑲_Ty K)) :
-        eval e δ = existT _ K v ->
+        (alts : forall (K : 𝑲 T), { x : 𝑿 & Stm (ctx_snoc Γ (x , 𝑲_Ty K)) τ}) :
         ⟨ δ , stm_match_union e alts ⟩ --->
-        ⟨ δ , stm_let' (env_nil ► projT1 (alts K)∶𝑲_Ty K ↦ untag v) (projT2 (alts K))  ⟩
+        ⟨ δ , let (K , v) := eval e δ in
+              stm_let' (env_nil ► projT1 (alts K)∶𝑲_Ty K ↦ untag v) (projT2 (alts K))
+        ⟩
     | step_stm_match_record
         (δ : LocalStore Γ) {R : 𝑹} {Δ : Ctx (𝑿 * Ty)}
         (e : Exp Γ (ty_record R)) (p : RecordPat (𝑹𝑭_Ty R) Δ)
@@ -484,7 +502,69 @@ Module Type ProgramKit (typeKit : TypeKit) (termKit : TermKit typeKit).
         ⟨ δ , stm_match_record R e p rhs ⟩ --->
         ⟨ δ , stm_let' (pattern_match p (eval e δ)) rhs ⟩
 
-    where "st₁ ---> st₂" := (@step _ _ st₁ st₂).
+    where "'⟨' δ1 ',' s1 '⟩' '--->' '⟨' δ2 ',' s2 '⟩'" := (@Step _ _ δ1 δ2 s1 s2).
+
+    Definition Final {Γ σ} (s : Stm Γ σ) : Prop :=
+      match s with
+      | stm_lit _ _  => True
+      | stm_exit _ _ => True
+      | _ => False
+      end.
+
+    Lemma can_form_store_cat (Γ Δ : Ctx (𝑿 * Ty)) (δ : LocalStore (Γ ▻▻ Δ)) :
+      exists (δ₁ : LocalStore Γ) (δ₂ : LocalStore Δ), δ = env_cat δ₁ δ₂.
+    Admitted.
+
+    Lemma can_form_store_snoc (Γ : Ctx (𝑿 * Ty)) (x : 𝑿) (σ : Ty) (δ : LocalStore (Γ ▻ (x , σ))) :
+      exists (δ' : LocalStore Γ) (v : Lit σ), δ = env_snoc δ' x σ v.
+    Admitted.
+
+    Lemma can_form_store_nil (δ : LocalStore ε) :
+      δ = env_nil.
+    Admitted.
+
+    Local Ltac progress_can_form :=
+      match goal with
+      | [ H: LocalStore (ctx_snoc _ _) |- _ ] => pose proof (can_form_store_snoc H)
+      | [ H: LocalStore ctx_nil |- _ ] => pose proof (can_form_store_nil H)
+      | [ H: LocalStore (ctx_cat _ _) |- _ ] => pose proof (can_form_store_cat _ _ H)
+      end; destruct_conjs; subst.
+
+    Local Ltac progress_simpl :=
+      repeat
+        (cbn in *; destruct_conjs; subst;
+         try progress_can_form;
+         try match goal with
+             | [ |- True \/ _] => left; constructor
+             | [ |- False \/ _] => right
+             | [ |- forall _, _ ] => intro
+             | [ H: True |- _ ] => clear H
+             | [ H: Final ?s |- _ ] => destruct s; cbn in H; try contradiction
+             | [ H : _ \/ _ |- _ ] => destruct H
+             end).
+
+    Local Ltac progress_inst T :=
+      match goal with
+      | [ IH: (forall (δ : LocalStore (ctx_cat ?Γ ?Δ)), _),
+          δ1: LocalStore ?Γ, δ2: LocalStore ?Δ |- _
+        ] => specialize (IH (env_cat δ1 δ2)); T
+      | [ IH: (forall (δ : LocalStore (ctx_snoc ctx_nil (?x , ?σ))), _),
+          v: Lit ?σ |- _
+        ] => specialize (IH (env_snoc env_nil x σ v)); T
+      | [ IH: (forall (δ : LocalStore ?Γ), _), δ: LocalStore ?Γ |- _
+        ] => solve [ specialize (IH δ); T | clear IH; T ]
+      end.
+
+    Local Ltac progress_tac :=
+      progress_simpl;
+      try solve
+          [ progress_inst progress_tac
+          | repeat eexists; constructor; eauto
+          ].
+
+    Lemma progress {Γ σ} (s : Stm Γ σ) :
+      Final s ∨ forall δ, exists δ' s', ⟨ δ , s ⟩ ---> ⟨ δ' , s' ⟩.
+    Proof. induction s; intros; progress_tac. Qed.
 
   End SmallStep.
 
